%iffalse
\let\negmedspace\undefined
\let\negthickspace\undefined
\documentclass[journal,12pt,twocolumn]{IEEEtran}
\usepackage{cite}
\usepackage{amsmath,amssymb,amsfonts,amsthm}
\usepackage{algorithmic}
\usepackage{graphicx}
\usepackage{textcomp}
\usepackage{xcolor}
\usepackage{txfonts}
\usepackage{listings}
\usepackage{enumitem}
\usepackage{mathtools}
\usepackage{gensymb}
\usepackage{comment}
\usepackage[breaklinks=true]{hyperref}
\usepackage{tkz-euclide} 
\usepackage{listings}
\usepackage{gvv}                                        
%\def\inputGnumericTable{}                                 
\usepackage[latin1]{inputenc}                                
\usepackage{color}                                            
\usepackage{array}                                            
\usepackage{longtable}                                       
\usepackage{calc}                                             
\usepackage{multirow}                                         
\usepackage{hhline}                                           
\usepackage{ifthen}                                           
\usepackage{lscape}
\usepackage{tabularx}
\usepackage{array}
\usepackage{float}


\newtheorem{theorem}{Theorem}[section]
\newtheorem{problem}{Problem}
\newtheorem{proposition}{Proposition}[section]
\newtheorem{lemma}{Lemma}[section]
\newtheorem{corollary}[theorem]{Corollary}
\newtheorem{example}{Example}[section]
\newtheorem{definition}[problem]{Definition}
\newcommand{\BEQA}{\begin{eqnarray}}
\newcommand{\EEQA}{\end{eqnarray}}
\newcommand{\define}{\stackrel{\triangle}{=}}
\theoremstyle{remark}
\newtheorem{rem}{Remark}
\begin{document}

\bibliographystyle{IEEEtran}
\vspace{3cm}

\title{11.9.3.17}
\author{EE23BTECH11017 - Eachempati Mihir Divyansh$^{*}$% <-this % stops a space
}
\maketitle
\newpage
\bigskip

\renewcommand{\thefigure}{\theenumi}
\renewcommand{\thetable}{\theenumi}

\textbf{Question: }
If the $4^{th}$, $10^{th}$ and $16^{th}$ terms of a G.P. are x, y, and z, respectively. Prove that $x,\; y,\; z$ are in G.P.


\begin{table}[h]
    \renewcommand\thetable{1}
    \centering
        \caption{\textbf{Given Information}}
    \begin{tabular}{|m{2cm}|m{2cm}|m{2cm}|}
    \hline
    \textbf{Symbol} & \textbf{Value} & \textbf{Description}\\ [1ex]
    \hline
        $x$ & $x\brak{0}r^4$ & $x\brak{4}$ \\ [1ex]
    \hline
        $y$ & $x\brak{0}r^{10}$ & $x\brak{10}$\\ [1ex]
    \hline
        $z$ & $x\brak{0}r^{16}$ & $x\brak{16}$\\ [1ex]
    \hline
        $r$ & $y^{\frac{1}{6}}x^{-\frac{1}{6}}$ & $\frac{x\brak{n}}{x\brak{n-1}}$\\[1ex]
    \hline \vspace{0.1cm}
        $x\brak{0}$ & $x^{\frac{5}{3}}y^{-\frac{2}{3}}$ & First term \\[1ex]
    \hline
        $x\brak{n}$ & $x\brak{0}r^nu\brak{n}$ & General Term \\ [1ex]
    \hline
    \end{tabular}\label{Table 1}
\end{table} 

\solution

\begin{enumerate}
\item From \tabref{Table 1},
\begin{align}
\notag x&= x\brak{4} =x\brak{0}r^4 \\
\notag y&=x\brak{10}=x\brak{0}r^{10} \\
\notag z&=x\brak{16}=x\brak{0}r^{16}
\end{align}
Consider $\dfrac{x\brak{10}}{x\brak{4}}$ and $\dfrac{x\brak{16}}{x\brak{10}}$;
\begin{align}
 \dfrac{x\brak{10}}{x\brak{4}} &= \dfrac{x\brak{0}r^{10}}{x\brak{0}r^4} = r^6\\ 
 \dfrac{x\brak{16}}{x\brak{10}} &= \dfrac{x\brak{0}r^{16}}{x\brak{0}r^{10}} = r^6
\end{align}
Since, $\dfrac{x\brak{10}}{x\brak{4}}$ = $\dfrac{x\brak{16}}{x\brak{10}}$;\\
\begin{align}  
\notag   & x\brak{4},\; x\brak{10},\; x\brak{16}\text{ are in G.P.} \\
\notag  \therefore & x,\; y,\; z \text{ are in G.P.}
\end{align}

\item
To extend the domain of n to -ve integers, the step function $u\brak{n}$ can be used.
\begin{align}
 \notag    \therefore x\brak{n} &= x\brak{0}r^n u\brak{n} \; \forall \;n\in Z
\end{align}

\item
$x\brak{0}$ and $r$ can be expressed in terms of $x$, $y$, and $z$ in the following manner.
\begin{align}
 \notag      x&=x\brak{0}r^4 \\
 \notag    \frac{y}{x}&=r^6 \\
 \Rightarrow r&=\sqrt[6]{\frac{y}{x}}=\brak{\frac{y}{x}}^{\frac{1}{6}}\\
 \notag    x\brak{0}&=\frac{x}{r^4}\\
 \notag    x\brak{0}&=x\brak{\frac{x}{y}}^{\frac{4}{6}}\\
 \therefore\; x\brak{0}&=x^{\frac{5}{3}}y^{-\frac{2}{3}} \\
 and\; r&=\brak{\frac{y}{x}}^{\frac{1}{6}}= y^{\frac{1}{6}}x^{-\frac{1}{6}}
\end{align}
\item 
Z-transform:    $x\brak{n} \system{Z} X\brak{z}$
\begin{align*}
    X\brak{z}&= \sum_{n=-\infty}^{\infty} x\brak{n}z^{-n}\\
    X\brak{z}&=\dfrac{x\brak{0}}{1-rz^{-1}}\: \forall\: |z|>|r|
\end{align*}
Substituting $r$ and $x\brak{0}$, 
\begin{align*}
     X\brak{z}&=\dfrac{x^{\frac{5}{3}}y^{-\frac{2}{3}}}{1-{\brak{\frac{y}{x}}^{\frac{1}{6}}}z^{-1}}
\end{align*}
\item Example 
\begin{align*}
    \text{Let}\;x\brak{0} =\dfrac{1}{256}\;\text{and}\;r = 2\\     x=x\brak{4}=x\brak{0}r^4 &=\frac{1}{256}\brak{2}^4=\frac{1}{16}\\
     x&=\frac{1}{16} \\
    y=x\brak{10}=x\brak{0}r^{10} &=\frac{1}{256}\brak{2}^{10}=4\\
     y&=4 \\
    z=x\brak{16}=x\brak{0}r^{16} &=\frac{1}{256}\brak{2}^{16}=256\\
     z&=256 \\
\end{align*}
\newpage
\begin{figure}[!h]
    \centering
    \renewcommand\thefigure{1}
   % \caption{Stem Plot of $x(n)$ vs $n$}
    \includegraphics[width=\columnwidth]{A_1.png}
        \label{fig:1}
\end{figure}


\end{enumerate}

\end{document}
